src/ModularArithmetic/ModularBaseSystemBasicInterface.v
@@ -1,0 +1,172 @@
+Require Import Crypto.BaseSystem.
+Require Import Crypto.ModularArithmetic.ModularBaseSystem.
+Require Import Crypto.ModularArithmetic.ModularBaseSystemProofs.
+Require Import Crypto.BaseSystemProofs.
+Require Import Crypto.Util.Tuple Crypto.Util.CaseUtil.
+Require Import ZArith.
+Require Import Crypto.Algebra.
+Import Group.
+Import PseudoMersenneBaseParams PseudoMersenneBaseParamProofs.
+
+(* Wraps ModularBaseSystem operations in tuples *)
+Generalizable All Variables.
+Section s.
+  Context `{prm:PseudoMersenneBaseParams m}.
+
+  Definition fe := tuple Z (length base).
+
+(* to have them in specific, we need them in interface. To put them in interface, we
+   need to either
+
+   a) define them in interface
+   b) define them in opt
+   c) define them in MBS
+   d) define them in some kind of tuple wrapper for MBS which we then later unfold
+
+abstractions:
+- Fq
+- MBS with list rep +length proofs
+- MBS with tuple rep
+    (do correctness of MBS here)
+- optimized MBS
+*)
+
+  Definition mul  (x y:fe) : fe :=
+    carry_mul k_ c (from_list_default 0%Z (length base))
+      (to_list _ x) (to_list _ y).
+
+  Definition add : fe -> fe -> fe.
+    refine (on_tuple2 add_opt _).
+    abstract (intros; rewrite add_opt_correct, add_length_exact; case_max; omega).
+  Defined.
+
+  Definition sub : fe -> fe -> fe.
+    refine (on_tuple2 sub_opt _).
+    abstract (intros; rewrite sub_opt_correct; apply length_sub; rewrite ?coeff_length; auto).
+  Defined.
+
+  Definition carry_simple i := fun us =>
+    let di := nth_default 0 us      i in
+    let us' := set_nth i (pow2_mod di (log_cap i)) us in
+    add_to_nth (S i) (   (Z.shiftr di (log_cap i))) us'.
+
+  Definition carry_and_reduce i := fun us =>
+    let di := nth_default 0 us      i in
+    let us' := set_nth i (pow2_mod di (log_cap i)) us in
+    add_to_nth   0  (c * (Z.shiftr di (log_cap i))) us'.
+
+  Definition carry i : digits -> digits :=
+    if eq_nat_dec i (pred (length base))
+    then carry_and_reduce i
+    else carry_simple i.
+
+  Definition carry_sequence is us := fold_right carry us is.
+
+  Fixpoint make_chain i :=
+    match i with
+    | O => nil
+    | S i' => i' :: make_chain i'
+    end.
+
+  Definition full_carry_chain := make_chain (length limb_widths).
+
+  Definition carry_full := carry_sequence full_carry_chain.
+
+  Definition carry_mul us vs := carry_full (mul us vs).
+
+End CarryBasePow2.
+
+Section Canonicalization.
+  Context `{prm :PseudoMersenneBaseParams}.
+
+  (* compute at compile time *)
+  Definition max_ones := Z.ones (fold_right Z.max 0 limb_widths).
+
+  Definition max_bound i := Z.ones (log_cap i).
+
+  Fixpoint isFull' us full i :=
+    match i with
+    | O => andb (Z.ltb (max_bound 0 - c) (nth_default 0 us 0)) full
+    | S i' => isFull' us (andb (Z.eqb (max_bound i) (nth_default 0 us i)) full) i'
+    end.
+
+  Definition isFull us := isFull' us true (length base - 1)%nat.
+
+  Fixpoint modulus_digits' i :=
+    match i with
+    | O => max_bound i - c + 1 :: nil
+    | S i' => modulus_digits' i' ++ max_bound i :: nil
+    end.
+
+  (* compute at compile time *)
+  Definition modulus_digits := modulus_digits' (length base - 1).
+
+  Definition and_term us := if isFull us then max_ones else 0.
+
+  Definition freeze us :=
+    let us' := carry_full (carry_full (carry_full us)) in
+    let and_term := and_term us' in
+    (* [and_term] is all ones if us' is full, so the subtractions subtract q overall.
+       Otherwise, it's all zeroes, and the subtractions do nothing. *)
+     map2 (fun x y => x - y) us' (map (Z.land and_term) modulus_digits).
+
+End Canonicalization.
+
+
+  Arguments to_list {_ _} _.
+  Definition phi (a : fe) : ModularArithmetic.F m := decode (to_list a).
+  Definition phi_inv (a : ModularArithmetic.F m) : fe :=
+    from_list_default 0%Z _ (encode a).
+
+  Lemma phi_inv_spec : forall a, phi (phi_inv a) = a.
+  Proof.
+    intros; cbv [phi_inv phi].
+    erewrite from_list_default_eq.
+    rewrite to_list_from_list.
+    apply ModularBaseSystemProofs.encode_rep.
+    Grab Existential Variables.
+    apply ModularBaseSystemProofs.encode_rep.
+  Qed.
+
+  Definition eq (x y : fe) : Prop := phi x = phi y.
+
+  Definition zero : fe := phi_inv (ModularArithmetic.ZToField 0).
+
+  Definition opp (x : fe) : fe := phi_inv (ModularArithmetic.opp (phi x)).
+
+  Lemma add_correct : forall a b,
+    to_list (add a b) = BaseSystem.add (to_list a) (to_list b).
+  Proof.
+    intros; cbv [add on_tuple2].
+    rewrite to_list_from_list.
+    apply add_opt_correct.
+  Qed.
+
+  Lemma add_phi : forall a b : fe,
+    phi (add a b) = ModularArithmetic.add (phi a) (phi b).
+  Proof.
+    intros; cbv [phi].
+    rewrite add_correct.
+    apply ModularBaseSystemProofs.add_rep; auto using decode_rep, length_to_list.
+  Qed.
+
+  Lemma mul_correct : forall a b,
+    to_list (mul a b) = carry_mul (to_list a) (to_list b).
+  Proof.
+    intros; cbv [mul].
+    rewrite carry_mul_opt_cps_correct by assumption.
+    erewrite from_list_default_eq.
+    apply to_list_from_list.
+    Grab Existential Variables.
+    apply carry_mul_length; apply length_to_list.
+  Qed.
+
+  Lemma mul_phi : forall a b : fe,
+    phi (mul a b) = ModularArithmetic.mul (phi a) (phi b).
+  Proof.
+    intros; cbv beta delta [phi].
+    rewrite mul_correct.
+    apply carry_mul_rep; auto using decode_rep, length_to_list.
+  Qed.
+
+End s.
